Split NRGTNF into defs and theory

src/NRGTNF.v
@@ -23,16 +23,13 @@ Require Import Ssromega.
 Section NRGTNF.
 
   Variables Name Vals : ordType.
-  Variable s : @wfSchema Name Vals.
+  Variables (s : @wfSchema Name Vals).
   
   Implicit Type queries : seq (@Query Name Vals).
   Implicit Type query : @Query Name Vals.
-  Notation is_field := (@is_field Name Vals).
-  Notation is_inline_fragment := (@Query.is_inline_fragment Name Vals).
-
-  Ltac apply_andP := apply/andP; split=> //.
-  Ltac apply_and3P := apply/and3P; split=> //.
-
+  
+  
+  
   
   Equations is_grounded query : bool  :=
     {
@@ -60,21 +57,9 @@ Section NRGTNF.
             are_grounded (q :: qs) := q.(is_grounded) && if q.(is_field) then are_grounded_fields qs else are_grounded_inlines qs
                                                                                                                               
           }.
-  
-      
-  Lemma are_grounded_fields_E qs : are_grounded_fields qs = all is_field qs && all is_grounded qs.
-  Proof.
-    elim: qs => //= q qs ->.
-      by rewrite andbACA -[RHS]andbA.
-  Qed.
-  
-  Lemma are_grounded_inlines_E qs : are_grounded_inlines qs = all is_inline_fragment qs && all is_grounded qs.
-  Proof.
-    elim: qs => //= q qs ->.
-      by rewrite andbACA -[RHS]andbA.
-  Qed.
+
  
-  Equations is_grounded2 (type_in_scope : @NamedType Name) (query : @Query Name Vals) : bool :=
+  Equations is_grounded2 (type_in_scope : Name) (query : @Query Name Vals) : bool :=
     {
       is_grounded2 ty (NestedField f _ φ)
         with lookup_field_in_type s ty f :=
@@ -95,7 +80,7 @@ Section NRGTNF.
       is_grounded2 _ _ := true
     }
    where
-   are_grounded2 (type_in_scope : @NamedType Name) (queries : seq (@Query Name Vals)) : bool :=
+   are_grounded2 (type_in_scope : Name) (queries : seq (@Query Name Vals)) : bool :=
      {
        are_grounded2 _ [::] := true;
        are_grounded2 ty (hd :: tl)
@@ -106,151 +91,7 @@ Section NRGTNF.
          }
      }.
 
-
-  Lemma are_grounded2_cat ty qs1 qs2 :
-    are_grounded2 ty (qs1 ++ qs2) = are_grounded2 ty qs1 && are_grounded2 ty qs2 .
-  Proof.
-    elim: qs1 => //= q qs1 IH.
-    by case is_object_type => /=; rewrite IH //=;
-    rewrite -[RHS]andbA -[(_ && are_grounded2 ty qs1) && are_grounded2 ty qs2]andbA.
-  Qed.
-
-  Lemma are_grounded2_consE ty q qs :
-    are_grounded2 ty (q :: qs) ->
-    are_grounded2 ty qs.
-  Proof.
-    by case: q => //= [f α | l f α | f α φ | l f α φ | t φ]; case: is_object_type => /=; case/and3P.
-  Qed.
-
-    
   
-   (*
-  
-   Lemma are_grounded_in_abstract_scope_are_any schema ty queries :
-     is_abstract_type schema ty ->
-     are_grounded_2 schema ty queries ->
-     all is_field queries \/ all is_inline_fragment queries.
-   Proof.
-     move=> Habs; rewrite are_grounded_2E.
-     rewrite abstract_type_N_obj //=.
-     by move/andP=> [/orP [/andP [_ Hinl] | /andP [_ Hflds]] _]; [right | left].
-   Qed.
-   
-   Lemma all_grounded_fields_in_object_scope_are_grounded schema ty queries :
-     is_object_type schema ty ->
-     all is_field queries ->
-     all (is_grounded_2 schema ty) queries ->
-     are_grounded_2 schema ty queries.
-   Proof.
-       by move=> Hobj; rewrite are_grounded_2E Hobj /= orbF => Hflds Hgs; apply/andP.
-   Qed.
-    *)
-
-   (* Lemma is_grounded_2_in_normal_form schema query :
-     forall ty,
-       query_conforms schema ty query ->
-       is_grounded_2 schema ty query ->
-       is_grounded query.
-   Proof.
-     elim query using Query_ind with
-         (Pl := fun qs =>
-                 forall ty,
-                   all (query_conforms schema ty) qs ->
-                   are_grounded_2 schema ty qs ->
-                   all (is_grounded) qs) => // [f α | l f α | t | hd IHhd tl IHtl ]; last first.
-     - move=> ty.
-       all_cons => [Hqc Hqsc] /=.
-       case: is_object_type => //=; [| case get_possible_types => //= [| hd' tl']]; move/and3P=> [Hty Hg Hgs];
-       by apply/andP; split; [apply: (IHhd ty) | apply: (IHtl ty)].
-       
-     all: do [move=> φ IH ty]; simp is_grounded_2; simp is_in_normal_form.
-
-     - simp query_conforms => /and5P [_ _ Hne Hqsc _] /and3P [Hobj Hflds Hg].
-       apply/and3P; split => //.
-       apply: (IH t) => //= {IH}.
-         by apply: all_grounded_fields_in_object_scope_are_grounded.
-
-     - move/nlf_conformsP=> [fld Hlook /and3P [/orP [Hobj | Habs] _]];
-       rewrite /queries_conform Hlook /= => /and3P [Hne Hqsc _] Hg; apply/andP.
-       * split.
-           by apply/orP; left; apply: (are_grounded_in_object_scope_are_fields schema fld.(return_type)).
-           by apply: (IH fld.(return_type)).
-
-       * split.
-           by apply/orP; apply: (are_grounded_in_abstract_scope_are_any schema fld.(return_type)).
-           by apply: (IH fld.(return_type)).
- 
-      - move/nf_conformsP=> [fld Hlook /and3P [/orP [Hobj | Habs] _]];
-       rewrite /queries_conform Hlook /= => /and3P [Hne Hqsc _] Hg; apply/andP.
-       * split.
-           by apply/orP; left; apply: (are_grounded_in_object_scope_are_fields schema fld.(return_type)).
-           by apply: (IH fld.(return_type)).
-
-       * split.
-           by apply/orP; apply: (are_grounded_in_abstract_scope_are_any schema fld.(return_type)).
-           by apply: (IH fld.(return_type)).
-   Qed.*)
-
-   Lemma grounded2_are_fields_in_object_scope :
-     forall ty qs,
-       is_object_type s ty ->
-       are_grounded2 ty qs ->
-       all is_field qs.
-   Proof.
-      apply (is_grounded2_elim
-              (fun ty q b => true)
-              (fun ty qs b =>
-                 is_object_type s ty ->
-                 b ->
-                 all is_field qs)) => //.
-      - by intros => /=; case/and3P: H2 => *; apply_andP; apply: H0.
-      - by intros; rewrite H1 in Heq.
-   Qed.
-
-
-   Lemma are_grounded2_are_grounded :
-     forall queries ty,
-       are_grounded2 ty queries ->
-       are_grounded queries.
-   Proof.
-     apply (is_grounded_elim 
-              (fun q b =>
-                 forall ty,
-                   is_grounded2 ty q ->
-                   b)
-              (fun qs b =>
-                 forall ty,
-                   is_object_type s ty ->
-                   are_grounded2 ty qs ->
-                   b)
-              (fun qs b =>
-                 forall ty,
-                   is_object_type s ty = false ->
-                   are_grounded2 ty qs ->
-                   b)
-              (fun qs b =>
-                 forall ty,
-                   are_grounded2 ty qs ->
-                   b)
-           ) => //=.
-     
-     - move=> f α φ IH ty; simp is_grounded2.
-       case lookup_field_in_type => //=; case; intros; apply: IH; exact: H.
-     - move=> l f α φ IH ty; simp is_grounded2.
-       case lookup_field_in_type => //=; case; intros; apply: IH; exact: H.
-     - by move=> t φ IH ty; simp is_grounded2 => /andP [Ht Hg]; apply_andP; apply: (IH t) => //.
-
-     - by move=> q qs IHq IHqs ty Hcond /=; rewrite Hcond /= => /and3P [Hf Hg Hgs]; apply_and3P; [ apply: (IHq ty) | apply: (IHqs ty)].
-     -  by move=> q qs IHq IHqs ty Hscope; rewrite Hscope /=; case/and3P=> *; apply_and3P; [apply: (IHq ty) | apply: (IHqs ty)].
-        
-     - move=> q qs IHq IHflds IHinls ty.
-       case Hscope : is_object_type => //= /and3P [Htype Hg Hgs].
-       * by rewrite Htype; apply_andP; [apply: (IHq ty) | apply: (IHflds ty)].
-       * have : forall q, q.(is_inline_fragment) -> q.(is_field) = false by case.
-         by move/(_ q Htype) ->; apply_andP; [apply : (IHq ty) | apply: (IHinls ty)].
-   Qed.
-
-   
   Equations are_similar (q1 q2 : @Query Name Vals) : bool :=
     {
       are_similar (InlineFragment t _) (InlineFragment t' _) := t == t';
@@ -277,7 +118,7 @@ Section NRGTNF.
     are_non_redundant query.(qsubqueries).
   
 
-
+  Definition are_in_normal_form queries := are_grounded queries && are_non_redundant queries.
 
 
   
@@ -293,3 +134,5 @@ Arguments are_non_redundant [Name Vals].
 Arguments is_non_redundant  [Name Vals].
 
 Arguments are_similar [Name Vals].
+
+Arguments are_in_normal_form [Name Vals].
