src/theory/NRGTNFLemmas.v
@@ -1,0 +1,129 @@
+From mathcomp Require Import all_ssreflect.
+Set Implicit Arguments.
+Unset Strict Implicit.
+Unset Printing Implicit Defensive.
+
+From Equations Require Import Equations.
+From extructures Require Import ord.
+
+
+Require Import Query.
+Require Import QueryAux.
+Require Import SchemaWellFormedness.
+
+Require Import Schema.
+Require Import SchemaAux.
+
+Require Import QueryConformance.
+
+Require Import SeqExtra.
+
+Require Import Ssromega.
+
+Require Import NRGTNF.
+
+Section Theory.
+
+  Ltac apply_andP := apply/andP; split=> //.
+  Ltac apply_and3P := apply/and3P; split=> //.
+
+  Variables (Name Vals : ordType).
+
+  Section Ground.
+    Variable (s : @wfSchema Name Vals).
+    
+    Lemma are_grounded_fields_E qs : are_grounded_fields s qs = all (fun q => q.(is_field)) qs && all (is_grounded s) qs.
+    Proof.
+      elim: qs => //= q qs ->.
+        by rewrite andbACA -[RHS]andbA.
+    Qed.
+    
+    Lemma are_grounded_inlines_E qs : are_grounded_inlines s qs = all (fun q => q.(is_inline_fragment)) qs && all (is_grounded s) qs.
+    Proof.
+      elim: qs => //= q qs ->.
+        by rewrite andbACA -[RHS]andbA.
+    Qed.
+
+    
+    Lemma are_grounded2_cat ty qs1 qs2 :
+      are_grounded2 s ty (qs1 ++ qs2) = are_grounded2 s ty qs1 && are_grounded2 s ty qs2 .
+    Proof.
+      elim: qs1 => //= q qs1 IH.
+        by case is_object_type => /=; rewrite IH //=;
+                                     rewrite -[RHS]andbA -[(_ && are_grounded2 s ty qs1) && are_grounded2 s ty qs2]andbA.
+    Qed.
+
+    Lemma are_grounded2_consE ty q qs :
+      are_grounded2 s ty (q :: qs) ->
+      are_grounded2 s ty qs.
+    Proof.
+        by case: q => //= [f α | l f α | f α φ | l f α φ | t φ]; case: is_object_type => /=; case/and3P.
+    Qed.
+
+    Lemma grounded2_are_fields_in_object_scope :
+      forall ty qs,
+        is_object_type s ty ->
+        are_grounded2 s ty qs ->
+        all (fun q => q.(is_field)) qs.
+    Proof.
+      apply (is_grounded2_elim Name Vals s
+               (fun ty q b => true)
+               (fun ty qs b =>
+                  is_object_type s ty ->
+                  b ->
+                  all (fun q => q.(is_field)) qs)) => //.
+      - by intros => /=; case/and3P: H2 => *; apply_andP; apply: H0.
+      - by intros; rewrite H1 in Heq.
+    Qed.
+
+
+    Lemma are_grounded2_are_grounded :
+      forall queries ty,
+        are_grounded2 s ty queries ->
+        are_grounded s queries.
+    Proof.
+      apply (is_grounded_elim Name Vals s
+               (fun q b =>
+                  forall ty,
+                    is_grounded2 s ty q ->
+                    b)
+               (fun qs b =>
+                  forall ty,
+                    is_object_type s ty ->
+                    are_grounded2 s ty qs ->
+                    b)
+               (fun qs b =>
+                  forall ty,
+                    is_object_type s ty = false ->
+                    are_grounded2 s ty qs ->
+                    b)
+               (fun qs b =>
+                  forall ty,
+                    are_grounded2 s ty qs ->
+                    b)
+            ) => //=.
+      
+      - move=> f α φ IH ty; simp is_grounded2.
+        case lookup_field_in_type => //=; case; intros; apply: IH; exact: H.
+      - move=> l f α φ IH ty; simp is_grounded2.
+        case lookup_field_in_type => //=; case; intros; apply: IH; exact: H.
+      - by move=> t φ IH ty; simp is_grounded2 => /andP [Ht Hg]; apply_andP; apply: (IH t) => //.
+
+      - by move=> q qs IHq IHqs ty Hcond /=; rewrite Hcond /= => /and3P [Hf Hg Hgs]; apply_and3P; [ apply: (IHq ty) | apply: (IHqs ty)].
+      -  by move=> q qs IHq IHqs ty Hscope; rewrite Hscope /=; case/and3P=> *; apply_and3P; [apply: (IHq ty) | apply: (IHqs ty)].
+         
+      - move=> q qs IHq IHflds IHinls ty.
+        case Hscope : is_object_type => //= /and3P [Htype Hg Hgs].
+        * by rewrite Htype; apply_andP; [apply: (IHq ty) | apply: (IHflds ty)].
+        * have : forall (q : @Query Name Vals), q.(is_inline_fragment) -> q.(is_field) = false by case.
+            by move/(_ q Htype) ->; apply_andP; [apply : (IHq ty) | apply: (IHinls ty)].
+    Qed.
+    
+  End Ground.
+
+  Section NonRedundant.
+
+  End NonRedundant.
+
+  
+End Theory.
